stack: prove simple, non-terminating clients.

src/example/TreiberClient02.v
@@ -20,7 +20,7 @@ Module TreiberClient2.
     Definition thread_push :
       ktree (threadE ident state) unit unit
       := fun _ =>
-      _ <- (trigger Yield;;; TreiberStack.push (s,SCMem.val_nat 0));;
+      _ <- (trigger Yield;;; TreiberStack.push (s,SCMem.val_nat 1));;
       Ret tt.
 
     Definition thread_pop :
@@ -70,505 +70,126 @@ Section SPEC.
   (* Namespace for TreiberClient2 invariants. *)
   Definition N_TreiberClient2 : namespace := (nroot .@ "Treiber" .@ "TreiberClient2").
 
-  Definition Clinet2StackState n γs γtok : sProp n :=
+  Definition Client2StackState n γs γtok : sProp n :=
     ((○ γs [SCMem.val_nat 1] ∗ ● γtok tt)∨ ○ γs ([] : list SCMem.val))%S.
 
-  Definition Client2Inv n γs γtok : sProp n :=
-    (syn_inv n N_TreiberClient2 (Clinet2StackState n γs γtok))%S.
+  Definition C2Inv n γs γtok : sProp n :=
+    (syn_inv n N_TreiberClient2 (Client2StackState n γs γtok))%S.
 
-  Global Instance Client2Inv_persistent n γs γtok : Persistent ⟦Client2Inv n γs γtok, n⟧.
+  Global Instance C2Inv_persistent n γs γtok : Persistent ⟦C2Inv n γs γtok, n⟧.
   Proof.
-    unfold Persistent. iIntros "H". unfold Client2Inv. rewrite red_syn_inv.
+    unfold Persistent. iIntros "H". unfold C2Inv. rewrite red_syn_inv.
     iDestruct "H" as "#H". auto.
   Qed.
 
   (** Simulation proof. *)
 
-  Lemma TreiberClient2_push_spec tid N :
-    ⊢ ∀ γs γtok (L : τ{nat, 1+N}) (ds : list (nat * nat * sProp N)),
-    [@ tid, N, ⊤ @]
+  Lemma TreiberClient2_push_spec tid n :
+    ⊢ ∀ γs γtok (L : τ{nat, 1+n}) (ds : list (nat * nat * sProp n)),
+    [@ tid, n, ⊤ @]
       ⧼⟦(
-        (syn_tgt_interp_as N sndl (fun m => s_memory_black m)) ∗
-        (⤉ IsTreiber N s γs) ∗
-        (⤉ Client2Inv N γs γtok) ∗
+        (syn_tgt_interp_as n sndl (fun m => s_memory_black m)) ∗
+        (⤉ IsTreiber n s γs) ∗
+        (⤉ C2Inv n γs γtok) ∗
         (⤉ ● γtok tt) ∗
         (⤉ Duty(tid) ds) ∗
         ◇{ds@1}(2+L, 2)
-        )%S, 1+N⟧⧽
+        )%S, 1+n⟧⧽
         (OMod.close_itree omod (SCMem.mod gvs) (thread_push tt))
-        ⧼_, ⟦(⤉ Duty(tid) ds)%S, 1+N⟧⧽
+        ⧼_, ⟦(⤉ Duty(tid) ds)%S, 1+n⟧⧽
   .
   Proof.
-    iIntros. iStartTriple. unfold Client2Inv.
-    red_tl_all. rewrite red_syn_tgt_interp_as; rewrite red_syn_inv; simpl.
-    iIntros "(#Mem & #IsTreiber & #Client2Inv & Tok & Duty & Pcs)".
+    iIntros. iStartTriple. unfold C2Inv.
+    red_tl_all. simpl. rewrite red_syn_tgt_interp_as;
+    rewrite red_syn_inv. simpl.
+    iIntros "(#Mem & #IsTreiber & #C2Inv & Tok & Duty & Pcs)".
+    simpl.
     iMod (pcs_decr _ _ 1 1 with "Pcs") as "[Pcs PcsPush]"; [lia|].
     iMod (pcs_drop _ _ _ _ 1 100 with "Pcs") as "Pcs"; [lia|].
-    iIntros "Post".
-    unfold thread_push. rred.
+    Unshelve. 2:lia.
+    iIntros "Post". unfold thread_push. rred.
     iApply (wpsim_yieldR2 with "[$Duty $Pcs]"); [lia..|].
-    iIntros "Duty _ Pcs". rred2r. iApply wpsim_tauR. rred2r.
+    iIntros "Duty _ Pcs". rred2r.
+    iApply wpsim_tauR. rred2r.
     iApply (Treiber_push_spec _ (λ v, ⌜ True ⌝)%S with "[Duty PcsPush Tok] [-]"); [ss..| |].
     { red_tl_all. rewrite red_syn_tgt_interp_as. iSplit; [eauto|]. iSplitR; [iFrame "#"|].
       iFrame. iIntros (s_st). red_tl_all. iIntros "[TStackInv _]".
       rewrite red_syn_fupd. red_tl_all.
-      iInv "Client2Inv" as "INV". "INV_CLOSE".
-      iMod (inv_ac "Client2Inv" as "INV" "INV_CLOSE".
-      iDestruct (auexa_b_w_eq with "TStackInv TStack") as "%EQ".
+      iInv "C2Inv" as "TStackC" "CloseC2Inv".
+      iEval (unfold Client2StackState; simpl; red_tl_all; simpl) in "TStackC".
+      (* Prove that the stack is empty. *)
+      iDestruct "TStackC" as "[[TStackC Tok'] | TStackC]".
+      { by iDestruct (auexa_b_b_false with "Tok Tok'") as %?. }
+      iDestruct (auexa_b_w_eq with "TStackInv TStackC") as "%EQ".
       subst s_st.
-      iMod (auexa_b_w_update with "TStackInv TStack") as "[TStackInv TStack]".
+      iMod (auexa_b_w_update with "TStackInv TStackC") as "[TStackInv TStackC]".
+      iMod ("CloseC2Inv" with "[TStackC Tok]") as "_".
+      { iEval (unfold Client2StackState; simpl; red_tl_all; simpl).
+        iLeft. iFrame.
+      }
       iModIntro. iFrame.
     }
-
-    iApply (Spinlock_lock_spec with "[LIVE_k Duty PcsPush] [-]").
-    1,2: ss.
-    { red_tl. rewrite red_syn_tgt_interp_as. iSplit. eauto. iSplitR. eauto. iFrame. }
-    Unshelve. 2: lia.
-    iEval (red_tl). iIntros (_) "[%γu A]". iEval (red_tl) in "A". iDestruct "A" as "[%u A]".
-    iEval (unfold counter; red_tl; simpl) in "A".
-    iDestruct "A" as "([%x A] & LOCKED & LIVE_k & Duty & LIVE_u & PC_u)". iEval (red_tl) in "A".
-    iDestruct "A" as "[%y A]". iEval (red_tl) in "A". iDestruct "A" as "(PT & CNTB_r1 & CNTB_r2)".
-    rred2r. iMod (pc_drop _ 1 _ _ 99 with "PC_u") as "PC_u". lia.
-    Unshelve. 2: lia.
-    iPoseProof (pcs_cons_fold with "[PC_u Pcs]") as "Pcs".
-    { simpl. iSplitR "Pcs". 2: iFrame. instantiate (1:=0). iFrame. }
-    iApply (wpsim_yieldR2 with "[Duty Pcs]").
-    3:{ iSplitL "Duty". iFrame. iFrame. }
-    auto. lia.
-    iIntros "Duty _ Pcs". iModIntro. rred2r.
-    iApply (SCMem_load_fun_spec with "[PT]").
-    3:{ iFrame. eauto. }
-    auto. ss.
-    iIntros (rv) "[%RV PT]". rred2r. iApply wpsim_tauR. rred2r.
-    iApply (wpsim_yieldR2 with "[Duty Pcs]").
-    3:{ iSplitL "Duty"; iFrame. }
-    auto. lia.
-    iIntros "Duty _ Pcs". iModIntro. rred2r.
-    iApply (SCMem_store_fun_spec with "[PT]").
-    3:{ iFrame. eauto. }
-    auto. ss.
-    iIntros (rv0) "PT". rred2r. iApply wpsim_tauR. rred2r.
-    iApply (wpsim_yieldR2 with "[Duty Pcs]").
-    3:{ iSplitL "Duty"; iFrame. }
-    auto. lia.
-    iIntros "Duty _ Pcs". iEval (simpl) in "Pcs". iModIntro. rred2r. iApply wpsim_tauR. rred2r.
-    destruct CASES as [CASE | CASE]; des; subst r0; subst c0.
-    - replace (SCMem.val_add rv c1) with ((c1 * (1 + x) + c2 * y) : SCMem.val).
-      2:{ subst rv. ss. f_equal. lia. }
-      iPoseProof (auexa_b_w_eq with "CNTB_r1 CNTW_r0") as "%EQ". subst a.
-      iMod (auexa_b_w_update _ _ _ _ nat (1 + x) with "CNTB_r1 CNTW_r0") as "[CNTB_r1 CNTW_r0]".
-      iMod (pcs_decr _ _ 1 1 with "Pcs") as "[Pcs _]". lia.
-      iApply (Spinlock_unlock_spec with "[CNTB_r1 CNTB_r2 PT LOCKED LIVE_k Duty Pcs LIVE_u PC_k]").
-      3:{ repeat (try rewrite @red_tl_sepconj). simpl.
-          iSplitR. rewrite red_syn_tgt_interp_as. eauto. iSplitR. eauto.
-          unfold counter. red_tl. iSplitL "PT CNTB_r1 CNTB_r2".
-          { iExists _. red_tl. iExists _. red_tl. iFrame. }
-          simpl. iFrame.
-      }
-      1,2: ss.
-      iEval red_tl. iIntros (_) "[Duty LIVE_k]". rred2r.
-      iApply "POST". replace (1+x) with (x+1). iFrame. lia.
-    - replace (SCMem.val_add rv c2) with ((c1 * x + c2 * (1 + y)) : SCMem.val).
-      2:{ subst rv. ss. f_equal. lia. }
-      iPoseProof (auexa_b_w_eq with "CNTB_r2 CNTW_r0") as "%EQ". subst a.
-      iMod (auexa_b_w_update _ _ _ _ nat (1 + y) with "CNTB_r2 CNTW_r0") as "[CNTB_r2 CNTW_r0]".
-      iMod (pcs_decr _ _ 1 1 with "Pcs") as "[Pcs _]". lia.
-      iApply (Spinlock_unlock_spec with "[CNTB_r1 CNTB_r2 PT LOCKED LIVE_k Duty Pcs LIVE_u PC_k]").
-      3:{ repeat (try rewrite @red_tl_sepconj). simpl.
-          iSplitR. rewrite red_syn_tgt_interp_as. eauto. iSplitR. eauto.
-          unfold counter. red_tl. iSplitL "PT CNTB_r1 CNTB_r2".
-          { iExists _. red_tl. iExists _. red_tl. iFrame. }
-          simpl. iFrame.
-      }
-      1,2: ss.
-      iEval red_tl. iIntros (_) "[Duty LIVE_k]". rred2r.
-      iApply "POST". replace (1+y) with (y+1). iFrame. lia.
-  Qed.
-
-  Local Opaque incr.
-
-  Lemma Client03_thread1_spec
-        tid N
-    :
-    ⊢ ⟦(∀ (r γk k γw w wl r1 r2 : τ{nat, 1+N}),
-           ((syn_tgt_interp_as N sndl (fun m => (➢ (scm_memory_black m))))
-              ∗ TID(tid)
-              ∗ (⤉ Duty(tid) [])
-              ∗ (⤉ isSpinlock N r L (counter N 2 5 r1 r2) γk k 4 2)
-              ∗ ➢(@live γk nat k (1/2))
-              ∗ ◇[k](3, 101)
-              ∗ ➢(auexa_w r1 0)
-              ∗ ◆[w, wl]
-              ∗ (⤉ t2_promise_inv N γw w r2)
-           )
-             -∗
-             syn_wpsim (1+N) tid ∅
-             (fun rs rt => (⤉(syn_term_cond N tid _ rs rt))%S)
-             false false
-             (fn2th Client03Spec.module "thread1" (tt ↑))
-             (fn2th Client03.module "thread1" (tt ↑)))%S, 1+N⟧.
-  Proof.
-    iIntros. simpl.
-    red_tl; iIntros (r). red_tl; iIntros (γk). red_tl. iIntros (k). red_tl. iIntros (γw).
-    red_tl. iIntros (w). red_tl. iIntros (wl). red_tl. iIntros (r1). red_tl. iIntros (r2).
-    red_tl. simpl.
-    rewrite red_syn_tgt_interp_as. unfold t2_promise_inv. rewrite red_syn_inv. rewrite red_syn_wpsim.
-    iIntros "(#MEM & TID & Duty & #ISL & LIVE_k & PC_k & CNTW_r1 & #LO_w & #UNTILI)".
-    unfold fn2th. simpl. lred2r. rred2r.
-    iApply (wpsim_yieldR with "[Duty]").
-    2:{ iSplitL "Duty". iApply "Duty". simpl. ss. }
-    auto.
-    iIntros "Duty _". iModIntro. rred2r. iApply wpsim_tauR. rred2r.
-    assert (exists j, 0 = j). eauto. des.
-    replace
-      (ITree.iter
-         (λ i : nat,
-             ` r0 : nat + () <- (if Nat.eq_dec i 100 then Ret (inr ()) else incr 2;;; trigger Yield;;; Ret (inl (i + 1)));; Ret r0)
-         0)
-      with
-      (ITree.iter
-         (λ i : nat,
-             ` r0 : nat + () <- (if Nat.eq_dec i 100 then Ret (inr ()) else incr 2;;; trigger Yield;;; Ret (inl (i + 1)));; Ret r0)
-         j).
-    2:{ subst j. auto. }
-    iEval (replace 250 with ((100 * 2) + 50)).
-    remember (100 - j) as J.
-    assert (100 = J). subst. ss.
-    iEval (rewrite H0) in "PC_k". iEval (rewrite H) in "CNTW_r1".
-    assert (LT : j <= 100). subst. lia.
-    clear H0 H.
-    iStopProof.
-    revert j HeqJ LT. induction J; cycle 1.
-    { i. iIntros "((#MEM & #ISL & #LO_w & #UNTILI) & TID & LIVE_k & PC_k & CNTW_r1 & Duty)".
-      iEval (rewrite unfold_iter_eq). rred2r.
-      destruct (Nat.eq_dec j 100).
-      { exfalso. lia. }
-      rred2.
-      iPoseProof (pc_split _ _ 1 (S J) with "PC_k") as "[PC_k1 PC_k]".
-      iApply (Client03_incr_spec with "[Duty LIVE_k PC_k1 CNTW_r1] [TID PC_k]").
-      ss.
-      { red_tl. simpl. iSplitR. rewrite red_syn_tgt_interp_as. eauto. iFrame.
-        simpl. iSplitR; [iApply pcs_nil |]. iSplit. eauto. iSplit; eauto.
-      }
-      iEval red_tl. iIntros (_) "(Duty & LIVE_k & CNTW_r1)". rred2r.
-      iApply (wpsim_yieldR with "[Duty]").
-      2:{ iSplitL "Duty". iApply "Duty". simpl. ss. }
-      auto.
-      iIntros "Duty _". iModIntro. rred2r. iApply wpsim_tauR. rred2r.
-      iApply wpsim_tauR.
-      specialize (IHJ (j+1)).
-      iPoseProof (IHJ with "[TID LIVE_k PC_k CNTW_r1 Duty]") as "IH".
-      { lia. }
-      { lia. }
-      { iSplit. iModIntro. eauto. iFrame. }
-      iApply "IH".
-    }
-    i. iIntros "((#MEM & #ISL & #LO_w & #UNTILI) & TID & LIVE_k & PC_k & CNTW_r1 & Duty)".
-    iEval (rewrite unfold_iter_eq). rred2r.
-    destruct (Nat.eq_dec j 100).
-    2:{ exfalso. lia. }
+    iEval (red_tl_all;simpl). iIntros (_) "[_ Duty]".
     rred2r.
-    (* Set-up for induction. *)
-    iEval (rewrite unfold_iter_eq). rred2r.
-    iApply (wpsim_yieldR with "[Duty]").
-    2:{ iFrame. }
-    auto.
-    iIntros "Duty _". iModIntro. rred2r.
-    iInv "UNTILI" as "UNTIL" "UNTIL_CLOSE".
-    iEval (unfold t2_promise; simpl; red_tl) in "UNTIL". iEval (rewrite red_syn_until_tpromise) in "UNTIL".
-    iPoseProof (until_tpromise_get_tpromise with "UNTIL") as "#TPROM".
-    iRevert "TID LIVE_k PC_k CNTW_r1 Duty UNTIL_CLOSE".
-    iMod (until_tpromise_ind with "[UNTIL] []") as "IH".
-    { iSplitR. eauto. iFrame. }
-    2:{ iApply "IH". }
-    iSplit; iModIntro.
-    { iIntros "IH". iModIntro. iIntros "CUR TID LIVE_k PC_k CNTW_r1 Duty UNTIL_CLOSE".
-      iEval (simpl; red_tl; simpl) in "CUR". iDestruct "CUR" as "[CUR0 CUR]".
-      iApply (SCMem_load_fun_spec with "[CUR] [-]").
-      3:{ iFrame. eauto. }
-      auto.
-      { rewrite lookup_insert. assert (↑N_state_tgt ## (↑N_t2_promise_inv : coPset)).
-        { apply ndot_preserve_disjoint_r. apply ndot_ne_disjoint. ss. }
-        set_solver.
-      }
-      iIntros (rv) "[%RVEQ PTD]". subst rv. rred2r. iApply wpsim_tauR. rred2r.
-      iMod ("UNTIL_CLOSE" with "[CUR0 PTD]") as "_".
-      { unfold t2_promise. simpl. rewrite red_syn_until_tpromise. iApply until_tpromise_make1. simpl. red_tl. iFrame. auto. }
-      iApply (wpsim_yieldR with "[Duty]").
-      2:{ iFrame. }
-      auto.
-      iIntros "Duty FC". iModIntro. rred2r. iApply (SCMem_compare_fun_spec with "[] [-]").
-      3:{ iApply tgt_interp_as_equiv. 2: eauto. ss. iIntros. red_tl.
-          ss. iSplit. iIntros "MEM"; iFrame. ss. iIntros "[MEM _]". iFrame.
-      }
-      auto. ss.
-      iIntros (rv) "[%TRUE _]". specialize (TRUE eq_refl). subst rv. rred2r. iApply wpsim_tauR.
-      rred2r. iApply wpsim_tauR.
-      iEval (rewrite unfold_iter_eq). rred2r.
-      iApply (wpsim_yieldR with "[Duty]").
-      2:{ iFrame. }
-      auto.
-      iIntros "Duty _". iModIntro. rred2r.
-      iInv "UNTILI" as "UNTIL" "UNTIL_CLOSE".
-      iEval (unfold t2_promise; simpl; red_tl) in "UNTIL". iEval (rewrite red_syn_until_tpromise) in "UNTIL".
-      iMod ("IH" with "[FC UNTIL]") as "IH".
-      { iFrame. }
-      iApply ("IH" with "TID LIVE_k PC_k CNTW_r1 Duty UNTIL_CLOSE").
-    }
-    { iIntros "#PR". iIntros "TID LIVE_k PC_k CNTW_r1 Duty UNTIL_CLOSE".
-      iMod ("UNTIL_CLOSE" with "[]") as "_".
-      { unfold t2_promise. simpl. rewrite red_syn_until_tpromise. iApply until_tpromise_make2. simpl. iSplit; eauto. }
-      iEval (unfold t2_write_inv; simpl; red_tl) in "PR". iEval (rewrite red_syn_inv) in "PR".
-      iDestruct "PR" as "[DEAD PR]".
-      iInv "PR" as "PRO" "PR_CLOSE". iEval (unfold t2_write; simpl; red_tl) in "PRO".
-      iDestruct "PRO" as "[RES PTD]".
-      iApply (SCMem_load_fun_spec with "[PTD] [-]").
-      3:{ iFrame. eauto. }
-      auto.
-      { rewrite lookup_insert. assert (↑N_state_tgt ## (↑N_t2_write_inv : coPset)).
-        { apply ndot_preserve_disjoint_r. apply ndot_ne_disjoint. ss. }
-        set_solver.
-      }
-      iIntros (rv) "[%RVEQ PTD]". subst rv. rred2r. iApply wpsim_tauR. rred2r.
-      iMod ("PR_CLOSE" with "[PTD RES]") as "_".
-      { unfold t2_write. simpl. red_tl. iFrame. }
-      iApply (wpsim_yieldR with "[Duty]").
-      2:{ iFrame. }
-      auto.
-      iIntros "Duty _". iModIntro. rred2r.
-      iApply (SCMem_compare_fun_spec with "[] [-]").
-      3:{ iApply tgt_interp_as_equiv. 2: eauto. ss. iIntros. red_tl.
-          ss. iSplit. iIntros "MEM"; iFrame. ss. iIntros "[MEM _]". iFrame.
-      }
-      auto. ss.
-      iIntros (rv) "[_ %FALSE]". exploit FALSE. ss. intros; subst. clear FALSE. rred2r.
-      iApply wpsim_tauR. rred2r.
-      iApply (wpsim_yieldR with "[Duty]").
-      2:{ iFrame. }
-      auto.
-      iIntros "Duty _". iModIntro. rred2r. iApply wpsim_tauR. rred2r.
-      iApply (Spinlock_lock_spec with "[LIVE_k Duty] [-]").
-      3:{ red_tl. iSplitR. rewrite red_syn_tgt_interp_as. eauto. iSplitR. eauto. iFrame. }
-      ss. ss.
-      iEval red_tl. iIntros (_) "[%γu POST]".
-      iEval (red_tl) in "POST". iDestruct "POST" as "[%u POST]".
-      iEval (red_tl; simpl) in "POST".
-      iDestruct "POST" as "(CNT & LOCK & LIVE_k & Duty & LIVE_u & PC_u)".
-      rred2r. iMod (pc_drop _ 1 _ _ 100 with "PC_u") as "PC_u".
-      auto. Unshelve. 2: auto.
-      iPoseProof (pcs_cons_fold u 0 [] 1 _ with "[PC_u]") as "Pcs".
-      { simpl. iFrame. }
-      iApply (wpsim_yieldR2 with "[Duty Pcs]").
-      3:{ iSplitL "Duty"; iFrame. }
-      auto. lia.
-      iIntros "Duty _ Pcs". iModIntro. rred2r.
-      iEval (unfold counter; red_tl) in "CNT". iDestruct "CNT" as "[%x CNT]".
-      iEval (red_tl) in "CNT". iDestruct "CNT" as "[%y CNT]".
-      iEval (red_tl) in "CNT". iDestruct "CNT" as "(PT & CNTB_r1 & CNTB_r2)".
-      iApply (SCMem_load_fun_spec with "[PT] [-]").
-      3:{ iFrame. eauto. }
-      auto. ss.
-      iIntros (rv) "[%RV PT]". rred2r. iApply wpsim_tauR. rred2r.
-      iApply (wpsim_yieldR2 with "[Duty Pcs]").
-      3:{ iSplitL "Duty"; done. }
-      auto. lia.
-      iIntros "Duty _ Pcs". iModIntro. rred2r. iApply wpsim_tauR. rred2r.
-      (* Get numbers. *)
-      iInv "PR" as "PRO" "PR_CLOSE". iEval (unfold t2_write; simpl; red_tl) in "PRO".
-      iDestruct "PRO" as "[RES PTD]".
-      iPoseProof (auexa_b_w_eq with "CNTB_r1 CNTW_r1") as "%EQ1". subst x.
-      iPoseProof (auexa_b_w_eq with "CNTB_r2 RES") as "%EQ2". subst y.
-      iMod ("PR_CLOSE" with "[PTD RES]") as "_".
-      { unfold t2_write. simpl. red_tl. iFrame. }
-      iMod (pcs_decr _ _ 1 1 _ with "Pcs") as "[Pcs _]". lia.
-      iApply (Spinlock_unlock_spec with "[CNTB_r1 CNTB_r2 PT LOCK LIVE_k Duty LIVE_u Pcs PC_k]").
-      3:{ repeat (try rewrite @red_tl_sepconj). simpl.
-          iSplitR. rewrite red_syn_tgt_interp_as. eauto. iSplitR. eauto.
-          unfold counter. red_tl. iSplitL "PT CNTB_r1 CNTB_r2".
-          { iExists 100. red_tl. iExists 10. red_tl. iFrame. }
-          simpl. iFrame. simpl. done.
-      }
-      1,2: ss.
-      iEval red_tl. iIntros (_) "[Duty LIVE_k]". rred2r.
-      iApply (wpsim_sync with "[Duty]").
-      2:{ iFrame. }
-      auto.
-      iIntros "Duty _". iModIntro. rred2r. iApply wpsim_tauR. rred2r. lred2r.
-      subst rv. simpl.
-      iApply wpsim_ret.
-      2:{ iModIntro. iFrame. auto. }
-      reflexivity.
-    }
+    iApply "Post". iFrame.
   Qed.
 
-  Lemma Client03_thread2_spec
-        tid N
-    :
-    ⊢ ⟦(∀ (r γk k γw w r1 r2 : τ{nat, 1+N}),
-           ((syn_tgt_interp_as N sndl (fun m => (➢ (scm_memory_black m))))
-              ∗ TID(tid)
-              ∗ (⤉ Duty(tid) [(w, 0, t2_write_inv N r2)])
-              ∗ (⤉ isSpinlock N r L (counter N 2 5 r1 r2) γk k 4 2)
-              ∗ ➢(@live γk nat k (1/2))
-              ∗ ◇[k](3, 11)
-              ∗ ➢(auexa_w r2 0)
-              ∗ ◇[w](6, 31)
-              ∗ ➢(@live γw nat w (1/2))
-              ∗ (⤉ t2_promise_inv N γw w r2)
-           )
-             -∗
-             syn_wpsim (1+N) tid ∅
-             (fun rs rt => (⤉(syn_term_cond N tid _ rs rt))%S)
-             false false
-             (fn2th Client03Spec.module "thread2" (tt ↑))
-             (fn2th Client03.module "thread2" (tt ↑)))%S, 1+N⟧.
+  Lemma TreiberClient2_pop_spec tid n :
+    ⊢ ∀ γs γtok (L : τ{nat, 1+n}) (ds : list (nat * nat * sProp n)),
+    [@ tid, n, ⊤ @]
+      ⧼⟦(
+        (syn_tgt_interp_as n sndl (fun m => s_memory_black m)) ∗
+        (⤉ IsTreiber n s γs) ∗
+        (⤉ C2Inv n γs γtok) ∗
+        (⤉ Duty(tid) ds) ∗
+        ◇{ds@1}(2+L, 2)
+        )%S, 1+n⟧⧽
+        (OMod.close_itree omod (SCMem.mod gvs) (thread_pop tt))
+      ⧼rv, ⟦(
+        ⌜ if rv is Some v then
+            v = SCMem.val_nat 1
+          else
+            True ⌝ ∗
+        (⤉ Duty(tid) ds)
+        )%S, 1+n⟧⧽
+  .
   Proof.
-    iIntros.
-    red_tl; iIntros (r). red_tl. iIntros (γk). red_tl. iIntros (k). red_tl. iIntros (γw).
-    red_tl. iIntros (w). red_tl. iIntros (r1). red_tl. iIntros (r2).
-    red_tl. rewrite red_syn_tgt_interp_as. unfold t2_promise_inv. rewrite red_syn_inv. rewrite red_syn_wpsim. simpl.
-    iIntros "(#MEM & TID & Duty & #ISL & LIVE_k & PC_k & CNTW_r2 & PC_w & LIVE_w & #UNTILI)".
-    unfold fn2th. simpl. lred2r. rred2r.
-    iMod (pcs_decr [(w, 0)] _ 30 1 with "[PC_w]") as "[PCS_w1 PCS_w2]".
-    2:{ iApply pcs_cons_fold. iSplitL "PC_w". iFrame. ss. }
-    auto.
-    iMod (pcs_drop _ _ _ _ 1 100 with "PCS_w2") as "PCS_w2".
-    lia. Unshelve. 2: lia.
-    iApply (wpsim_yieldR2 with "[Duty PCS_w2]").
-    3:{ iSplitL "Duty". iApply "Duty". iFrame. }
-    auto. lia.
-    iIntros "Duty _ PCS_w2". iEval (simpl) in "PCS_w2". iModIntro. rred2r.
-    iApply wpsim_tauR. rred2r.
-    assert (exists j, 0 = j). eauto. des.
-    replace
-      (ITree.iter
-         (λ i : nat,
-             ` r0 : nat + () <- (if Nat.eq_dec i 10 then Ret (inr ()) else incr 5;;; trigger Yield;;; Ret (inl (i + 1)));; Ret r0)
-         0)
-      with
-      (ITree.iter
-         (λ i : nat,
-             ` r0 : nat + () <- (if Nat.eq_dec i 10 then Ret (inr ()) else incr 5;;; trigger Yield;;; Ret (inl (i + 1)));; Ret r0)
-         j).
-    2:{ subst j. auto. }
-    iEval (replace 50 with (5 * 10)).
-    remember (10 - j) as J.
-    assert (10 = J). subst. ss.
-    iPoseProof (pc_split_le _ _ J 1 with "PC_k") as "[PC_k PC_k2]". subst; lia.
-    iMod (pcs_decr _ _ (3*J) 0 with "PCS_w1") as "[PCS_w1 _]". subst; lia.
-    iEval (rewrite H) in "CNTW_r2".
-    assert (LT : j <= 10). subst. lia.
-    clear H0 H.
-    iStopProof.
-    revert j HeqJ LT. induction J; cycle 1.
-    { i. iIntros "((#MEM & #ISL & #UNTILI) & TID & LIVE_k & CNTW_r2 & LIVE_w & Duty & PCS_w1 & PC_k & PC_k1 & PCS_w)".
-      iPoseProof (pc_split_le _ _ 1 J with "PC_k") as "[PC_k0 PC_k]". lia.
-      iMod (pcs_decr _ _ 3 (3*J) with "PCS_w") as "[PCS_w0 PCS_w]". lia.
-      iMod (pcs_decr _ _ 2 1 with "PCS_w0") as "[PCS_w0 PCS_w2]". lia.
-      iEval (rewrite unfold_iter_eq). rred2r.
-      destruct (Nat.eq_dec j 10).
-      { exfalso. lia. }
-      rred2.
-      iApply (Client03_incr_spec with "[Duty PCS_w0 LIVE_k PC_k0 CNTW_r2] [-]").
-      ss.
-      { red_tl. simpl. iSplitR. rewrite red_syn_tgt_interp_as. eauto.
-        iSplitL "Duty". iFrame. iSplitL "PCS_w0". iFrame. iSplitR. eauto. iFrame.
-        iSplit; eauto.
-      }
-      iEval red_tl. iIntros (_) "(Duty & LIVE_k & CNTW_r1)". rred2r.
-      iMod (pcs_drop _ _ _ _ 1 1 with "PCS_w2") as "PCS_w2". lia. Unshelve. 2: auto.
-      iApply (wpsim_yieldR with "[Duty PCS_w2]").
-      2:{ iSplitL "Duty". iApply "Duty". iFrame. }
-      auto.
-      iIntros "Duty _". iModIntro. rred2r. iApply wpsim_tauR. rred2r. iApply wpsim_tauR.
-      specialize (IHJ (j+1)).
-      iPoseProof (IHJ with "[-]") as "IH".
-      { lia. }
-      { lia. }
-      { iSplit. iModIntro. eauto. iFrame. }
-      iApply "IH".
+    iIntros. iStartTriple. unfold C2Inv.
+    red_tl_all. simpl. rewrite red_syn_tgt_interp_as; rewrite red_syn_inv; simpl.
+    iIntros "(#Mem & #IsTreiber & #C2Inv & Duty & Pcs)".
+    iMod (pcs_decr _ _ 1 1 with "Pcs") as "[Pcs PcsPush]"; [lia|].
+    iMod (pcs_drop _ _ _ _ 1 100 with "Pcs") as "Pcs"; [lia|].
+    Unshelve. 2:lia.
+    iIntros "Post". unfold thread_pop. rred.
+    iApply (wpsim_yieldR2 with "[$Duty $Pcs]"); [lia..|].
+    iIntros "Duty _ Pcs". rred2r. iApply wpsim_tauR. rred2r.
+    iApply (Treiber_pop_spec _ (λ ov, ⌜ if ov is Some v then v = 1 else True ⌝)%S with "[Duty PcsPush] [-]"); [ss..| |].
+    { red_tl_all. rewrite red_syn_tgt_interp_as. iSplit; [eauto|]. iSplitR; [iFrame "#"|].
+      iFrame. iIntros (s_st). red_tl_all. iIntros "[TStackInv _]".
+      rewrite red_syn_fupd. red_tl_all.
+      iInv "C2Inv" as "TStackC" "CloseC2Inv".
+      iEval (unfold Client2StackState; simpl; red_tl_all; simpl) in "TStackC".
+      (* Case analysis on the current state of the stack. *)
+      iDestruct "TStackC" as "[[TStackC Tok] | TStackC]".
+      all: iDestruct (auexa_b_w_eq with "TStackInv TStackC") as "%EQ".
+      all: subst s_st; red_tl_all.
+      - iMod (auexa_b_w_update with "TStackInv TStackC") as "[TStackInv TStackC]".
+        iMod ("CloseC2Inv" with "[TStackC]") as "_".
+        { iEval (unfold Client2StackState; simpl; red_tl_all; simpl).
+          iRight. iFrame.
+        }
+        iModIntro. iFrame. done.
+      - iMod ("CloseC2Inv" with "[TStackC]") as "_".
+        { iEval (unfold Client2StackState; simpl; red_tl_all; simpl).
+          iRight. iFrame.
+        }
+        iModIntro. iFrame.
     }
-    i. iIntros "((#MEM & #ISL & #UNTILI) & TID & LIVE_k & CNTW_r2 & LIVE_w & Duty & PCS_w & _ & PC_k & _)".
-    iEval (rewrite unfold_iter_eq). rred2r. destruct (Nat.eq_dec j 10).
-    2:{ exfalso. lia. }
-    rred2r. iApply (wpsim_yieldR2 with "[Duty PCS_w]").
-    3:{ iSplitL "Duty". iFrame. iFrame. }
-    1,2: lia.
-    iIntros "Duty _ PCS_w". iEval (simpl) in "PCS_w". iModIntro. rred2r.
-    iInv "UNTILI" as "UNTIL" "UNTIL_CLOSE". iEval (unfold t2_promise; simpl; red_tl) in "UNTIL".
-    iEval (rewrite red_syn_until_tpromise) in "UNTIL". iDestruct "UNTIL" as "[#PR [L | D]]".
-    2:{ iEval (unfold t2_write_inv; simpl; red_tl; simpl) in "D". iPoseProof "D" as "#[D WI]".
-        iExFalso. iPoseProof (Lifetime.pending_not_shot with "LIVE_w D") as "%S". auto.
-    }
-    iEval (simpl; red_tl; simpl) in "L". iDestruct "L" as "[LIVE_w2 PTD]".
-    iApply (SCMem_store_fun_spec with "[PTD] [-]").
-    3:{ iSplitR. auto. iFrame. }
-    auto.
-    { rewrite lookup_insert. assert (↑N_state_tgt ## (↑N_t2_promise_inv : coPset)).
-      { apply ndot_preserve_disjoint_r. apply ndot_ne_disjoint. ss. }
-      set_solver.
-    }
-    iIntros (rv) "PTD". destruct rv. rred2r. iApply wpsim_tauR. rred2r.
-    iMod (Lifetime.pending_shot with "[LIVE_w LIVE_w2]") as "#DEAD_w".
-    { iEval (rewrite <- (Qp.div_2 1)). iApply (Lifetime.pending_merge with "LIVE_w LIVE_w2"). }
-    subst j. clear LT HeqJ.
-    iMod (FUpd_alloc _ _ _ _ N_t2_write_inv ((➢(auexa_w r2 (10:nat)) ∗ (D ↦ 1))%S : sProp N) with "[CNTW_r2 PTD]") as "#DONE".
-    2:{ simpl. red_tl. iFrame. }
-    auto.
-    iMod ("UNTIL_CLOSE" with "[]") as "_".
-    { simpl. unfold t2_promise. rewrite red_syn_until_tpromise. iSplitR. auto.
-      simpl; red_tl. simpl. iRight. iModIntro. auto.
-    }
-    iMod (duty_fulfill with "[Duty]") as "Duty".
-    { iSplitL. iFrame. simpl. auto. }
-    iApply (wpsim_yieldR with "[Duty]"). 2: iFrame. auto. iIntros "Duty _". iModIntro. rred2r.
-    iApply wpsim_tauR. rred2r. iApply (Spinlock_lock_spec with "[LIVE_k Duty] [-]").
-    3:{ red_tl. iSplitR. rewrite red_syn_tgt_interp_as. auto. iSplitR. eauto.  iFrame. }
-    1,2: ss.
-    iEval (red_tl). iIntros (_) "[%γu Q]". iEval (red_tl) in "Q". iDestruct "Q" as "[%u Q]".
-    iEval (red_tl; simpl) in "Q".
-    iDestruct "Q" as "(CNT & LOCK & LIVE_k & Duty & LIVE_u & PC_u)". rred2r.
-    iMod (pc_drop _ 1 _ _ 100 with "PC_u") as "PC_u". auto. Unshelve. 2: lia.
-    iPoseProof (pcs_cons_fold _ 0 [] 1 with "[PC_u]") as "Pcs".
-    { iFrame. }
-    iApply (wpsim_yieldR2 with "[Duty Pcs]").
-    3:{ iSplitL "Duty"; iFrame. }
-    1,2: lia.
-    iIntros "Duty _ Pcs". iEval (simpl) in "Pcs". iModIntro. rred2r.
-    iEval (unfold counter; red_tl) in "CNT". iDestruct "CNT" as "[%x CNT]".
-    iEval (red_tl) in "CNT". iDestruct "CNT" as "[%y CNT]".
-    iEval (red_tl) in "CNT". iDestruct "CNT" as "(PTC & CB_r1 & CB_r2)".
-    iApply (SCMem_load_fun_spec with "[PTC] [-]").
-    3:{ iSplitR. auto. iFrame. }
-    1,2: ss.
-    iIntros (rv) "[%RV PTC]". rred2r. iApply wpsim_tauR. rred2r.
-    iApply (wpsim_yieldR2 with "[Duty Pcs]").
-    3:{ iSplitL "Duty"; iFrame. }
-    1,2: lia.
-    iIntros "Duty _ Pcs". iEval (simpl) in "Pcs". iModIntro. rred2r. iApply wpsim_tauR. rred2r.
-    (* Get the value of y. *)
-    iInv "DONE" as "D" "D_CLOSE". iEval (simpl; red_tl; simpl) in "D". iDestruct "D" as "[W PT]".
-    iPoseProof (auexa_b_w_eq with "CB_r2 W") as "%EQ".
-    iMod ("D_CLOSE" with "[W PT]") as "_".
-    { simpl. red_tl. iFrame. }
-    iMod (pcs_decr _ _ 1 0 _ with "Pcs") as "[Pcs _]". lia.
-    iApply (Spinlock_unlock_spec with "[CB_r1 CB_r2 PTC LOCK LIVE_k Duty Pcs LIVE_u PC_k] [-]").
-    3:{ repeat (try rewrite @red_tl_sepconj). simpl.
-        iSplitR. rewrite red_syn_tgt_interp_as. eauto. iSplitR. eauto.
-        unfold counter. red_tl. iSplitL "PTC CB_r1 CB_r2".
-        { iExists _. red_tl. iExists _. red_tl. iFrame. }
-        simpl. iFrame. iFrame.
-    }
-    1,2: ss.
-    iEval red_tl. iIntros (_) "[Duty LIVE_k]". rred2r.
-    iApply wpsim_yieldL. lred2r. iApply wpsim_chooseL. iExists x. lred2r.
-    iApply (wpsim_sync with "[Duty]").
-    2:{ iFrame. }
-    auto.
-    iIntros "Duty _". iModIntro. rred2r. iApply wpsim_tauR. rred2r. lred2r.
-    subst y rv. iApply wpsim_ret.
-    2:{ iModIntro. iFrame. ss. }
-    reflexivity.
+    iIntros (ov). red_tl_all. iIntros "[%Hrv Duty]".
+
+    iEval (red_tl_all;simpl).
+    rred2r.
+    iApply "Post". red_tl_all. iFrame. done.
   Qed.
 
 End SPEC.
